Veir/Rewriter/WellFormed/Builder/OpRegion.lean
@@ -4,9 +4,12 @@ import Veir.Rewriter.Basic
 
 namespace Veir
 
+variable {dT : Type} [HasProperties dT]
+variable {ctx : IRContext dT}
+
 set_option warn.sorry false in
 theorem Rewriter.initOpRegions_WellFormed (opPtr: OperationPtr)
-    (hop : opPtr.InBounds ctx) (hctx : IRContext.WellFormed ctx) {hn} (newCtx : IRContext):
+    (hop : opPtr.InBounds ctx) (hctx : IRContext.WellFormed ctx) {hn} (newCtx : IRContext dT):
     Rewriter.initOpRegions ctx opPtr regions n hop regionInBounds (by grind) hn = some newCtx →
     newCtx.WellFormed := by
   sorry
